theories/LogicalRelation/Definition/Helper.v
@@ -39,7 +39,7 @@ Section PolyRed.
       shpRed [Δ] (ρ : Δ ≤ Γ) : [ |- Δ ] -> [ LogRel@{i j k l} l | Δ ||- shp⟨ρ⟩ ≅ shp'⟨ρ⟩ ] ;
       posRed [Δ a b] (ρ : Δ ≤ Γ) (wfΔ : [ |- Δ ]) :
           [ shpRed ρ wfΔ | Δ ||- a ≅ b : shp⟨ρ⟩] ->
-          WLRAdequate@{i j k l} Δ l pos[a .: (ρ >> tRel)] pos'[b .: (ρ >> tRel)] }.
+          WLRAdequate@{i j k l} Δ l pos⟨wk_up shp ρ⟩[a..] pos'⟨wk_up shp' ρ⟩[b..] }.
 
   Definition from@{i j k l} {PA : PolyRedPack@{k l} Γ shp shp' pos pos'}
     (PAad : PolyRedPackAdequate@{k l} (LogRel@{i j k l} l) PA)
@@ -242,115 +242,6 @@ Module SigRedTy.
 End SigRedTy.
 
 
-(* Inductive isLRPair' `{GenericTypingProperties}
-  {l Γ A B} (ΣA : [ Γ ||-Σ< l > A ≅ B ]) : term -> Type :=
-| PairLRPair' : forall (A' B' a b : term)
-      (wtydom : [Γ |- A'])
-      (convtydom : [Γ |- SigRedTy.domL ΣA ≅ A'])
-      (wtycod : [Γ |- B'[a..]])
-      (convtycod : [Γ |- (SigRedTy.codL ΣA)[a..] ≅ B'[a..]])
-  (rfst : forall {Δ} (ρ : Δ ≤ Γ) (wfΔ : [ |- Δ ]),
-      [ Δ ||-S< l > a⟨ρ⟩ ≅ a⟨ρ⟩ : (SigRedTy.domL ΣA)⟨ρ⟩ | ΣA.(PolyRed.shpRed) ρ wfΔ])
-  (rsnd : forall {Δ} (ρ : Δ ≤ Γ) (wfΔ : [ |- Δ ]),
-      [ wfΔ ||-< l > b⟨ρ⟩ ≅ b⟨ρ⟩ : (SigRedTy.codL ΣA)[a⟨ρ⟩ .: (ρ >> tRel)] | ΣA.(PolyRed.posRed) ρ wfΔ (rfst ρ wfΔ)]),
-
-  isLRPair' ΣA (tPair A' B' a b)
-
-| NeLRPair' : forall p : term, [Γ |- p ~ p : SigRedTy.outTy ΣA] -> isLRPair' ΣA p.
-
-
-Module SigRedTmEq'.
-
-  Record SigRedTm' `{GenericTypingProperties} {Γ l A B}
-    (ΣA :  [ Γ ||-Σ< l > A ≅ B ]) (t : term) : Type := Build_SigRedTm'
-      { nf : term;
-        red : [Γ |-[ ta ] t :⤳*: nf : SigRedTy.outTy ΣA];
-        ispair : isLRPair' ΣA nf }.
-  Arguments nf { _ _ _ _ _ _ _ _ _ _ _ _ _ _ _ _}.
-
-  Record SigRedTmEq' `{GenericTypingProperties} {Γ l A B}
-    (ΣA :  [ Γ ||-Σ< l > A ≅ B ]) (t u : term) : Type := Build_SigRedTmEq'
-    { redL : SigRedTm' ΣA t;
-      redR : SigRedTm' ΣA u;
-      eq : [Γ |- redL.(nf) ≅ redR.(nf) : SigRedTy.outTy ΣA];
-      eqFst : forall (Δ : context) (ρ : Δ ≤ Γ) (wfΔ : [ |- Δ]),
-        [ _ ||-S< l > tFst redL.(nf)⟨ρ⟩ ≅ tFst redR.(nf)⟨ρ⟩ : _ | PolyRed.shpRed ΣA ρ wfΔ ];
-      eqSnd : forall (Δ : context) (ρ : Δ ≤ Γ) (wfΔ : [ |- Δ]),
-        [ _ ||-< l > tSnd redL.(nf)⟨ρ⟩ ≅ tSnd redR.(nf)⟨ρ⟩ : _ | PolyRed.posRed ΣA ρ wfΔ (eqFst Δ ρ wfΔ)]
-    }.
-
-  Definition whred `{GenericTypingProperties} {Γ l A B} {ΣA : [ Γ ||-Σ< l > A ≅ B ]} {t} :
-    SigRedTm' ΣA t -> [Γ |- t ↘  SigRedTy.outTy ΣA].
-  Proof.
-    intros [?? ispair]; econstructor; tea.
-    destruct ispair; constructor; now eapply convneu_whne.
-  Defined.
-
-  Definition whredL `{GenericTypingProperties} {Γ l A B} {ΣA : [ Γ ||-Σ< l > A ≅ B ]} {t u} :
-    SigRedTmEq' ΣA t u -> [Γ |- t ↘  SigRedTy.outTy ΣA ].
-  Proof. intros []; now eapply whred. Defined.
-
-  Definition whredR `{GenericTypingProperties} {Γ l A B} {ΣA : [ Γ ||-Σ< l > A ≅ B ]} {t u} :
-    SigRedTmEq' ΣA t u -> [Γ |- u ↘  SigRedTy.outTy ΣA ].
-  Proof. intros []; now eapply whred. Defined.
-
-End SigRedTmEq'.
-
-Export SigRedTmEq'(SigRedTm', Build_SigRedTm', SigRedTmEq', Build_SigRedTmEq').
-
-Lemma isLRPair_to `{GenericTypingProperties} {Γ l A B p} (ΣA : [ Γ ||-Σ< l > A ≅ B ]) : isLRPair' ΣA p -> isLRPair ΣA p.
-Proof.
-  intros.
-  induction X.
-  2: now econstructor.
-  now unshelve eapply PairLRPair.
-Defined.
-Lemma isLRPair_from `{GenericTypingProperties} {Γ l A B p} (ΣA : [ Γ ||-Σ< l > A ≅ B ]) : isLRPair ΣA p -> isLRPair' ΣA p.
-Proof.
-  intros.
-  induction X.
-  2: now econstructor.
-  now unshelve eapply PairLRPair'.
-Defined.
-
-Definition SigRedTm_to `{GenericTypingProperties} {Γ l A B}
-  (ΣA :  [ Γ ||-Σ< l > A ≅ B ]) (t : term) :
-  SigRedTm' ΣA t -> SigRedTm ΣA t.
-Proof.
-  intros [].
-  eapply isLRPair_to in ispair.
-  unshelve econstructor; tea.
-Defined.
-
-Definition SigRedTm_from `{GenericTypingProperties} {Γ l A B}
-  (ΣA :  [ Γ ||-Σ< l > A ≅ B ]) (t : term) :
-  SigRedTm ΣA t -> SigRedTm' ΣA t.
-Proof.
-  intros [].
-  eapply isLRPair_from in ispair.
-  unshelve econstructor; tea.
-Defined.
-
-Definition SigRedTmEq_to `{GenericTypingProperties} {Γ l A B}
-  (ΣA :  [ Γ ||-Σ< l > A ≅ B ]) (t u : term) :
-  SigRedTmEq' ΣA t u -> SigRedTmEq ΣA t u.
-Proof.
-  intros [].
-  unshelve econstructor; tea.
-  1,2: eapply SigRedTm_to; tea.
-  all: tea.
-Defined.
-
-Definition SigRedTmEq_from `{GenericTypingProperties} {Γ l A B}
-  (ΣA :  [ Γ ||-Σ< l > A ≅ B ]) (t u : term) :
-  SigRedTmEq ΣA t u -> SigRedTmEq' ΣA t u.
-Proof.
-  intros [].
-  unshelve econstructor; tea.
-  1,2: eapply SigRedTm_from; tea.
-  all: tea.
-Defined.
- *)
 Notation "[ Γ ||-Σ t ≅ u : A | ΣA ]" := (SigRedTmEq (Γ:=Γ) (A:=A) ΣA t u).
 
 #[program]
