theories/LogicalRelation/Introductions/SimpleArr.v
@@ -8,36 +8,42 @@ Set Printing Primitive Projection Parameters.
 Section SimpleArrow.
   Context `{GenericTypingProperties}.
 
-  Lemma shiftPolyRed {Γ}  {l A A' B B'} : [Γ ||-S<l> A ≅ A'] -> [Γ ||-S<l> B ≅ B'] -> PolyRed Γ l A A' B⟨↑⟩ B'⟨↑⟩.
+  Lemma shiftPolyRed {Γ}  {l A A' B B'} : [Γ ||-S<l> A ≅ A'] -> [Γ ||-S<l> B ≅ B'] ->
+    PolyRed Γ l A A' B⟨@wk1 Γ A⟩ B'⟨@wk1 Γ A'⟩.
   Proof.
     intros; escape; unshelve econstructor.
     - intros; now eapply SwkLR.
-    - intros; rewrite 2!shift_subst_scons; now eapply WAd_return, SwkLR.
+    - intros. rewrite <- 2wk_up_wk1, 2shift_subst1.
+      now eapply WAd_return, SwkLR.
   Qed.
 
-  Lemma ArrRedTy0 {Γ l A A' B B'} : [Γ ||-S<l> A ≅ A'] -> [Γ ||-S<l> B ≅ B'] -> [Γ ||-Π<l> arr A B ≅ arr A' B'].
+  Lemma ArrRedTy0 {Γ l A A' B B'} : [Γ ||-S<l> A ≅ A'] -> [Γ ||-S<l> B ≅ B'] ->
+    [Γ ||-Π<l> arr' Γ A B ≅ arr' Γ A' B'].
   Proof.
     intros RA RB.
     eapply LRPiPoly0, shiftPolyRed; tea; escape; gtyping.
   Qed.
 
-  Lemma SArrRedTy {Γ l A A' B B'} : [Γ ||-S<l> A ≅ A'] -> [Γ ||-S<l> B ≅ B'] -> [Γ ||-S<l> arr A B ≅ arr A' B'].
+  Lemma SArrRedTy {Γ l A A' B B'} : [Γ ||-S<l> A ≅ A'] -> [Γ ||-S<l> B ≅ B'] ->
+    [Γ ||-S<l> arr' Γ A B ≅ arr' Γ A' B'].
   Proof. intros; eapply LRPi'; now eapply ArrRedTy0. Qed.
 
-  Lemma ArrRedTy {Γ l A A' B B'} : [Γ ||-<l> A ≅ A'] -> [Γ ||-<l> B ≅ B'] -> [Γ ||-<l> arr A B ≅ arr A' B'].
+  Lemma ArrRedTy {Γ l A A' B B'} : [Γ ||-<l> A ≅ A'] -> [Γ ||-<l> B ≅ B'] ->
+    [Γ ||-<l> arr' Γ A B ≅ arr' Γ A' B'].
   Proof. 
     intros RA RB.
     eapply (Split_bind RA).
     intros Δ wfΔ ρ oRA.
     eapply (Split_wk_bind_return RB wfΔ ρ).
     intros Ξ wfΞ ρΞ oRB.
-    rewrite <- 2wk_arr.
+    rewrite <- 2wk_arr'.
     eapply SArrRedTy.
     + now eapply RA, overtree_PSh.
     + now eapply RB.
   Qed.
 
-  Lemma polyRedArrExt {Γ l A A' B B' C C'} : PolyRed Γ l A A' B B' -> PolyRed Γ l A A' C C' -> PolyRed Γ l A A' (arr B C) (arr B' C').
+  Lemma polyRedArrExt {Γ l A A' B B' C C'} : PolyRed Γ l A A' B B' ->
+    PolyRed Γ l A A' C C' -> PolyRed Γ l A A' (arr' (Γ,,A) B C) (arr' (Γ,,A') B' C').
   Proof.
     intros [RA RB] [RA' RC]; unshelve econstructor.
     1: eapply RA.
@@ -50,7 +56,7 @@ Section SimpleArrow.
     eapply WAdrefold.
     eapply (Split_wk_bind_return RC wfΞ ρΞ).
     intros Θ wfΘ ρΘ oRC.
-    rewrite 2!subst_arr, 2!wk_comp_ren_on, <-2!wk_arr.
+    rewrite <- 2wk_arr', <- 2!(Weakening.subst_arr' (Δ:=Δ)), 2!wk_comp_ren_on, <-2!wk_arr'.
     eapply SArrRedTy.
     + now eapply RB, overtree_PSh.
     + now eapply RC.
@@ -59,7 +65,7 @@ Section SimpleArrow.
   Lemma Ssimple_appcongTerm {Γ t t' u u' F F' G G' l}
     {RF : [Γ ||-S<l> F ≅ F']}
     (RG : [Γ ||-<l> G ≅ G'])
-    (RΠ : [Γ ||-S<l> arr F G ≅ arr F' G'])
+    (RΠ : [Γ ||-S<l> arr' Γ F G ≅ arr' Γ F' G'])
     (Rtt' : [Γ ||-S<l> t ≅ t' : _ | RΠ])
     (Ruu' : [Γ ||-S<l> u ≅ u' : F | RF ]) :
       [Γ ||-<l> tApp t u ≅ tApp t' u' : G | RG].
@@ -71,7 +77,7 @@ Section SimpleArrow.
   Lemma simple_appcongTerm {Γ t t' u u' F F' G G' l}
     {RF : [Γ ||-<l> F ≅ F']}
     (RG : [Γ ||-<l> G ≅ G'])
-    (RΠ : [Γ ||-<l> arr F G ≅ arr F' G'])
+    (RΠ : [Γ ||-<l> arr' Γ F G ≅ arr' Γ F' G'])
     (Rtt' : [Γ ||-<l> t ≅ t' : _ | RΠ])
     (Ruu' : [Γ ||-<l> u ≅ u' : F | RF ]) :
       [Γ ||-<l> tApp t u ≅ tApp t' u' : G | RG].
@@ -81,13 +87,13 @@ Section SimpleArrow.
     eapply (dSplit_wk_bind Rtt' wfΔ ρ).
     intros ??? oRΠ oRtt'.
     eapply Split_hom_PSh, (Wpackrefold wfΞ).
-    1: intros Θ wfΘ ρΘ h oRG; rewrite wk_comp_assoc; eapply h.
+    1:{ intros Θ wfΘ ρΘ h; rewrite wk_comp_assoc; eapply h. }
     rewrite <- 2!wk_app.
     unshelve eapply Ssimple_appcongTerm, Ruu', overtree_PSh, oRuu'; tea.
-    1: rewrite 2!wk_arr; now eapply RΠ, oRΠ.
+    1: rewrite 2!wk_arr'; now eapply RΠ, oRΠ.
     1: now eapply overtree_PSh.
     unshelve eapply SirrLREq, Rtt'; tea.
-    now bsimpl.
+    now rewrite wk_arr'.
   Qed.
 
 End SimpleArrow.
